Added definitions and lemmas to `cppmm.thy'.

cppmm.thy
@@ -184,84 +184,229 @@ datatype location_kind =
   | Non_atomic
   | Atomic
 
+
+(* Candidate execution, additionally defined by Cryolite *)
+types threads = "thread_id set"
+
+types actions = "action set"
+
+types location_typing = "location => location_kind"
+
+types sequenced_before = "action * action => bool"
+
+types additional_synchronized_with = "action * action => bool"
+
+types data_dependency = "action * action => bool"
+
+types control_dependency = "action * action => bool"
+
+types reads_from = "action * action => bool"
+
+types sequential_consistency = "action * action => bool"
+
+types modification_order = "action * action => bool"
+
+datatype "candidate_execution" =
+  Candidate_execution "threads"
+                      "actions"
+                      "location_typing"
+                      "sequenced_before"
+                      "additional_synchronized_with"
+                      "data_dependency"
+                      "control_dependency"
+                      "reads_from"
+                      "sequential_consistency"
+                      "modification_order"
+
+(* Accessor functions for candidate execution*)
+definition threads_of where
+  "threads_of x ==
+     (case x of Candidate_execution ts _ _ _ _ _ _ _ _ _ => ts)"
+
+definition actions_of where
+  "actions_of x ==
+     (case x of Candidate_execution _ as _ _ _ _ _ _ _ _ => as)"
+
+definition location_typing_of where
+  "location_typing_of x ==
+     (case x of Candidate_execution _ _ lt _ _ _ _ _ _ _ => lt)"
+
+definition sequenced_before_of where
+  "sequenced_before_of x ==
+     (case x of Candidate_execution _ _ _ sb _ _ _ _ _ _ => sb)"
+
+definition additional_synchronized_with_of where
+  "additional_synchronized_with_of x ==
+     (case x of Candidate_execution _ _ _ _ asw _ _ _ _ _ => asw)"
+
+definition data_dependency_of where
+  "data_dependency_of x ==
+     (case x of Candidate_execution _ _ _ _ _ dd _ _ _ _ => dd)"
+
+definition control_dependency_of where
+  "control_dependency_of x ==
+     (case x of Candidate_execution _ _ _ _ _ _ cd _ _ _ => cd)"
+
+definition reads_from_of where
+  "reads_from_of x ==
+     (case x of Candidate_execution _ _ _ _ _ _ _ rf _ _ => rf)"
+
+definition sequential_consistency_of where
+  "sequential_consistency_of x ==
+     (case x of Candidate_execution _ _ _ _ _ _ _ _ sc _ => sc)"
+
+definition modification_order_of where
+  "modification_order_of x ==
+     (case x of Candidate_execution _ _ _ _ _ _ _ _ _ mo => mo)"
+
+
+(* N3132 6.7 Location kinds (contd.) *)
 definition actions_respect_location_kinds where
-  "actions_respect_location_kinds actions location_kind_of ==
-     (ALL a : actions.
+  "actions_respect_location_kinds ce ==
+     (ALL a : (actions_of ce).
         (case location_of a of
            Some l =>
-             (case location_kind_of l of
+             (case (location_typing_of ce) l of
                 Mutex => is_lock_or_unlock a
               | Non_atomic => is_load_or_store a
               | Atomic => (is_load_or_store a | is_atomic_action a))
          | None => True))"
 
 definition is_at_location_kind where
-  "is_at_location_kind a (lk0::location_kind) location_kind_of ==
+  "is_at_location_kind ce a lk0 ==
      (case location_of a of
-        Some l => (location_kind_of l = lk0)
+        Some l => (location_typing_of ce l = lk0)
       | None => False)"
 
 definition is_at_mutex_location where
-  "is_at_mutex_location a location_kind_of == is_at_location_kind a Mutex location_kind_of"
+  "is_at_mutex_location ce a == is_at_location_kind ce a Mutex"
 
 definition is_at_non_atomic_location where
-  "is_at_non_atomic_location a location_kind_of == is_at_location_kind a Non_atomic location_kind_of"
+  "is_at_non_atomic_location ce a == is_at_location_kind ce a Non_atomic"
 
 definition is_at_atomic_location where
-  "is_at_atomic_location a location_kind_of == is_at_location_kind a Atomic location_kind_of"
+  "is_at_atomic_location ce a == is_at_location_kind ce a Atomic"
 
 
 (* N3132 6.8 Well-formed threads *)
 definition same_thread where
   "same_thread a b == (thread_id_of a = thread_id_of b)"
 
+(* same_thread as a binary relation, added by Cryolite *)
+definition same_thread_rel where
+  "same_thread_rel == (%(a, b). same_thread a b)"
+
 definition threadwise_relation_over where
-  "threadwise_relation_over s rel == (relation_over s rel & (ALL (a, b) : rel. (same_thread a b)))"
+  "threadwise_relation_over s rel ==
+     (relation_over s rel & (ALL (a, b) : rel. (same_thread_rel (a, b))))"
 
 definition same_location where
   "same_location a b == (location_of a = location_of b)"
 
+(* same_location_rel as a binary relation, added by Cryolite *)
+definition same_location_rel where
+  "same_location_rel == (%(a, b). same_location a b)"
+
 definition locations_of where
-  "locations_of actions == {l. (EX a : actions. (location_of a = Some l))}"
+  "locations_of as ==
+     {l. (EX a : as. (location_of a = Some l))}"
 
 definition well_formed_action where
   "well_formed_action a ==
      (case a of
-        (Atomic_load _ _ mem_ord _ _) => (mem_ord : {Mo_relaxed, Mo_acquire, Mo_seq_cst, Mo_consume})
-      | (Atomic_store _ _ mem_ord _ _) => (mem_ord : {Mo_relaxed, Mo_release, Mo_seq_cst})
-      | (Atomic_rmw _ _ mem_ord _ _ _) => (mem_ord : {Mo_relaxed, Mo_release, Mo_acquire, Mo_acq_rel, Mo_seq_cst, Mo_consume})
+        Atomic_load _ _ mem_ord _ _
+          => (mem_ord : {Mo_relaxed, Mo_acquire, Mo_seq_cst, Mo_consume})
+      | Atomic_store _ _ mem_ord _ _
+          => (mem_ord : {Mo_relaxed, Mo_release, Mo_seq_cst})
+      | Atomic_rmw _ _ mem_ord _ _ _
+          => (mem_ord : {Mo_relaxed, Mo_release, Mo_acquire, Mo_acq_rel, Mo_seq_cst, Mo_consume})
       | _ => True)"
 
 definition well_formed_threads where
-  "well_formed_threads threads actions location_kind_of sb asw dd cd ==
-     (inj_on action_id_of actions &
-      (ALL a : actions. well_formed_action a) &
-      threadwise_relation_over actions sb &
-      threadwise_relation_over actions dd &
-      threadwise_relation_over actions cd &
-      strict_preorder sb &
-      strict_preorder dd &
-      strict_preorder cd &
-      relation_over actions asw &
-      (ALL a : actions. (thread_id_of a : threads)) &
-      actions_respect_location_kinds actions location_kind_of &
-      dd <= sb)"
+  "well_formed_threads ce ==
+     (inj_on action_id_of (actions_of ce) &
+      (ALL a : (actions_of ce). well_formed_action a) &
+      threadwise_relation_over (actions_of ce) (sequenced_before_of ce) &
+      threadwise_relation_over (actions_of ce) (data_dependency_of ce) &
+      threadwise_relation_over (actions_of ce) (control_dependency_of ce) &
+      strict_preorder (sequenced_before_of ce) &
+      strict_preorder (data_dependency_of ce) &
+      strict_preorder (control_dependency_of ce) &
+      relation_over (actions_of ce) (additional_synchronized_with_of ce) &
+      (ALL a : (actions_of ce). (thread_id_of a : (threads_of ce))) &
+      actions_respect_location_kinds ce &
+      (data_dependency_of ce) <= (sequenced_before_of ce))"
+
+lemma same_thread_equiv: "equiv UNIV same_thread_rel"
+proof
+  have 10: "ALL a : UNIV. thread_id_of a = thread_id_of a" by blast
+  hence 20: "ALL a : UNIV. same_thread a a" by (unfold same_thread_def) blast
+  hence 30: "ALL a : UNIV. same_thread_rel (a, a)" by (unfold same_thread_rel_def) force
+  hence 40: "ALL a : UNIV. (a, a) : same_thread_rel" by (unfold mem_def)
+  have 50: "same_thread_rel <= UNIV" by blast
+  have 60: "UNIV <= UNIV <*> UNIV" by (unfold UNIV_Times_UNIV) blast
+  with 50 have 70: "same_thread_rel <= UNIV <*> UNIV" by blast
+  with 40 show 80: "refl_on UNIV same_thread_rel" by (unfold refl_on_def) blast
+next
+  have 90: "ALL a b. (thread_id_of a = thread_id_of b) --> (thread_id_of b = thread_id_of a)" by force
+  hence 100: "ALL a b. same_thread a b --> same_thread b a" by (unfold same_thread_def) blast
+  hence 110: "ALL a b. same_thread_rel (a, b) --> same_thread_rel (b, a)" by (unfold same_thread_rel_def) force
+  hence 120: "ALL a b. ((a, b) : same_thread_rel) --> ((b, a) : same_thread_rel)" by (unfold mem_def) blast
+  thus 130: "sym same_thread_rel" by (unfold sym_def) blast
+next
+  have 140: "ALL a b c. (thread_id_of a = thread_id_of b) -->
+                        (thread_id_of b = thread_id_of c) --> (thread_id_of a = thread_id_of c)" by force
+  hence 150: "ALL a b c. same_thread a b --> same_thread b c --> same_thread a c" by (unfold same_thread_def) blast
+  hence 160: "ALL a b c. same_thread_rel (a, b) --> same_thread_rel (b, c) --> same_thread_rel (a, c)"
+    by (unfold same_thread_rel_def) force
+  hence 170: "ALL a b c. ((a, b) : same_thread_rel) --> ((b, c) : same_thread_rel) --> ((a, c) : same_thread_rel)"
+    by (unfold mem_def) blast
+  thus 180: "trans same_thread_rel" by (unfold trans_def) blast
+qed
 
 
 (* N3132 6.9 Well-formed reads-from mapping *)
+
 definition well_formed_reads_from_mapping where
-  "well_formed_reads_from_mapping actions location_kind_of rf ==
-     (relation_over actions rf &
-      (ALL a : actions. (ALL aa : actions. (ALL b : actions. ((rf (a, b) & rf (aa, b)) --> (a = aa))))) &
-      (ALL (a, b) : rf.
-         (same_location a b &
+  "well_formed_reads_from_mapping ce ==
+     (relation_over (actions_of ce) (reads_from_of ce) &
+      (ALL a. ALL aa. ALL b. reads_from_of ce (a, b) & reads_from_of ce (aa, b) --> (a = aa)) &
+      (ALL (a, b) : (reads_from_of ce).
+         (same_location_rel (a, b) &
           (value_read b = value_written a) &
           (a ~= b) &
-          (is_at_mutex_location a location_kind_of --> (is_unlock a & is_lock b)) &
-          (is_at_non_atomic_location a location_kind_of --> (is_store a & is_load b)) &
-          (is_at_atomic_location a location_kind_of -->
+          (is_at_mutex_location ce a --> (is_unlock a & is_lock b)) &
+          (is_at_non_atomic_location ce a --> (is_store a & is_load b)) &
+          (is_at_atomic_location ce a -->
              ((is_atomic_store a | is_atomic_rmw a | is_store a)
               & (is_atomic_load b | is_atomic_rmw b | is_load b))))))"
+
+(* `read_by', which is the converse of `reads_from', added by Cryolite *)
+definition read_by_of where "read_by_of ce == converse (reads_from_of ce)"
+
+lemma read_by_is_single_valued: "well_formed_reads_from_mapping ce --> single_valued (read_by_of ce)"
+proof
+  assume 10: "well_formed_reads_from_mapping ce"
+  hence 20: "ALL a. ALL aa. ALL b. reads_from_of ce (a, b) & reads_from_of ce (aa, b) --> (a = aa)"
+    by (unfold well_formed_reads_from_mapping_def) blast
+  have 30: "((reads_from_of ce)^-1)^-1 = reads_from_of ce" by (rule converse_converse)
+  with 20 have 40: "ALL a. ALL aa. ALL b.
+                    (((reads_from_of ce)^-1)^-1) (a, b) & (((reads_from_of ce)^-1)^-1) (aa, b) --> (a = aa)"
+    by (unfold 30) blast
+  hence 60: "ALL a. ALL aa. ALL b.
+             (((a, b) : (((reads_from_of ce)^-1)^-1)) & ((aa, b) : (((reads_from_of ce)^-1)^-1))) --> (a = aa)"
+    by (unfold mem_def) blast
+  hence 60: "ALL a. ALL aa. ALL b.
+             (((b, a) : ((reads_from_of ce)^-1)) & ((b, aa) : ((reads_from_of ce)^-1))) --> (a = aa)"
+    by blast
+  hence 70: "ALL a. ALL aa. ALL b. (((b, a) : (read_by_of ce)) & ((b, aa) : (read_by_of ce))) --> (a = aa)"
+    by (unfold read_by_of_def) blast
+  hence 80: "ALL b. ALL a. ALL aa. (((b, a) : (read_by_of ce)) & ((b, aa) : (read_by_of ce))) --> (a = aa)" by blast
+  hence 90: "ALL b. ALL a. ALL aa. ((b, a) : (read_by_of ce)) --> ((b, aa) : (read_by_of ce)) --> (a = aa)" by blast
+  hence 100: "ALL b. ALL a. ((b, a) : (read_by_of ce)) --> (ALL aa. ((b, aa) : (read_by_of ce)) --> (a = aa))"
+    by blast
+  thus 110: "single_valued (read_by_of ce)" by (unfold single_valued_def) blast
+qed
 
 
 (* N3132 6.10 Consistent locks *)
@@ -270,14 +415,14 @@ definition all_lock_or_unlock_actions_at where
      {a : as. (is_lock_or_unlock a & (location_of a = lopt))}"
 
 definition consistent_locks where
-  "consistent_locks actions location_kind_of sc ==
-     (ALL l : locations_of actions. ((location_kind_of l = Mutex) --> (
-        let lock_unlock_actions = all_lock_or_unlock_actions_at(Some l) actions in
-        let lock_order = relation_int lock_unlock_actions sc in
+  "consistent_locks ce ==
+     (ALL l : locations_of (actions_of ce). ((location_typing_of ce l = Mutex) --> (
+        let lock_unlock_actions = all_lock_or_unlock_actions_at(Some l) (actions_of ce) in
+        let lock_order = relation_int lock_unlock_actions (sequential_consistency_of ce) in
         strict_total_order_over lock_unlock_actions lock_order &
         (ALL au : lock_unlock_actions. (is_unlock au -->
            (EX al : lock_unlock_actions.
-              (adjacent_less lock_order al au & same_thread al au & is_lock al)))) &
+              (adjacent_less lock_order al au & same_thread_rel (al, au) & is_lock al)))) &
         (ALL al : lock_unlock_actions. (is_lock al -->
            (ALL au : lock_unlock_actions.
               (adjacent_less lock_order au al --> is_unlock au)))))))"
@@ -285,190 +430,182 @@ definition consistent_locks where
 
 (* N3132 6.11 Release sequences *)
 definition rs_element where
-  "rs_element rs_head a == (same_thread a rs_head | is_atomic_rmw a)"
+  "rs_element rs_head a == (same_thread_rel (a, rs_head) | is_atomic_rmw a)"
 
 definition release_sequence where
-  "release_sequence ap location_kind_of mo ==
-     let (arel, b) = ap in
-     (is_at_atomic_location b location_kind_of &
-      is_release arel & (
-        (b = arel) |
-        (rs_element arel b & mo (arel, b) &
-           (ALL c. ((mo (arel, c) & mo (c, b)) -->
-              rs_element arel c)))))"
+  "release_sequence ce ==
+     (%(arel, b).
+      (is_at_atomic_location ce b &
+       is_release arel & (
+         (b = arel) |
+         (rs_element arel b & modification_order_of ce (arel, b) &
+            (ALL c. ((modification_order_of ce (arel, c) & modification_order_of ce (c, b)) -->
+               rs_element arel c))))))"
 
 definition hypothetical_release_sequence where
-  "hypothetical_release_sequence ap location_kind_of mo ==
-     let (a, b) = ap in
-     (is_at_atomic_location b location_kind_of & (
-        (b = a) |
-        (rs_element a b & mo (a, b) &
-           (ALL c. ((mo (a, c) & mo (c, b)) --> rs_element a c)))))"
+  "hypothetical_release_sequence ce ==
+     (%(a, b).
+      (is_at_atomic_location ce b & (
+         (b = a) |
+         (rs_element a b & modification_order_of ce (a, b) &
+            (ALL c. ((modification_order_of ce (a, c) & modification_order_of ce (c, b)) --> rs_element a c))))))"
 
 
 (* N3132 6.12 Synchronizes-with *)
 definition synchronizes_with where
-  "synchronizes_with ap actions location_kind_of sb asw rf sc mo ==
-     let (a, b) = ap in
-     (asw (a, b) |
-      (same_location a b & (a : actions) & (b : actions) & (
-         (is_unlock a & is_lock b & sc (a, b))                                                |
+  "synchronizes_with ce ==
+     (%(a, b).
+      (additional_synchronized_with_of ce (a, b) |
+       (same_location_rel (a, b) & (a : (actions_of ce)) & (b : (actions_of ce)) & (
+          (is_unlock a & is_lock b & sequenced_before_of ce (a, b))                          |
 
-         (is_release a & is_acquire b & ~(same_thread a b) &
-            (EX c. release_sequence (a, c) location_kind_of mo & rf (c, b)))                  |
+          (is_release a & is_acquire b & ~(same_thread_rel (a, b)) &
+             (EX c. release_sequence ce (a, c) & reads_from_of ce (c, b)))                  |
 
-         (is_fence a & is_release a & is_fence b & is_acquire b &
-            (EX x. EX y. same_location x y &
-               is_atomic_action x & is_atomic_action y & is_write x &
-               sb (a, x) & sb (y, b) &
-               (EX z. hypothetical_release_sequence (x, z) location_kind_of mo & rf (z, y)))) |
+          (is_fence a & is_release a & is_fence b & is_acquire b &
+             (EX x. EX y. same_location_rel (x, y) &
+                is_atomic_action x & is_atomic_action y & is_write x &
+                sequenced_before_of ce (a, x) & sequenced_before_of ce (y, b) &
+                (EX z. hypothetical_release_sequence ce (x, z) & reads_from_of ce (z, y)))) |
 
-         (is_fence a & is_release a & is_atomic_action b & is_acquire b &
-            (EX x. same_location x b &
-               is_atomic_action x & is_write x &
-               sb (a, x) &
-               (EX z. hypothetical_release_sequence (x, z) location_kind_of mo & rf (z, b)))) |
+          (is_fence a & is_release a & is_atomic_action b & is_acquire b &
+             (EX x. same_location_rel (x, b) &
+                is_atomic_action x & is_write x &
+                sequenced_before_of ce (a, x) &
+                (EX z. hypothetical_release_sequence ce (x, z) & reads_from_of ce (z, b)))) |
 
-         (is_atomic_action a & is_release a & is_fence b & is_acquire b &
-            (EX x. same_location a x & is_atomic_action x &
-               sb (x, b) &
-               (EX z. release_sequence (a, z) location_kind_of mo & rf (z, x)))))))"
+          (is_atomic_action a & is_release a & is_fence b & is_acquire b &
+             (EX x. same_location_rel (a, x) & is_atomic_action x &
+                sequenced_before_of ce (x, b) &
+                (EX z. release_sequence ce (a, z) & reads_from_of ce (z, x))))))))"
 
 
 (* N3132 6.13 Carries-a-dependency-to *)
 definition carries_a_dependency_to where
-  "carries_a_dependency_to ap sb dd rf ==
-     let ((a::action), b) = ap in
-     (((rf Int sb) Un dd)^*) (a, b)"
+  "carries_a_dependency_to ce ==
+     (%(a, b).
+      ((((reads_from_of ce) Int (sequenced_before_of ce)) Un (data_dependency_of ce))^*) (a, b))"
 
 
 (* N3132 6.14 Dependency-ordered-before *)
 definition dependency_ordered_before where
-  "dependency_ordered_before ap actions location_kind_of sb dd rf mo ==
-     let (a, d) = ap in
-     ((a : actions) & (d : actions) &
-       (EX b. (is_release a & is_consume b &
-          (EX e. (release_sequence (a, e) location_kind_of mo & rf (e, b))) &
-          (carries_a_dependency_to (b, d) sb dd rf | (b = d)))))"
+  "dependency_ordered_before ce ==
+     (%(a, d).
+      (a : (actions_of ce)) & (d : (actions_of ce)) &
+        (EX b. (is_release a & is_consume b &
+           (EX e. (release_sequence ce (a, e) & reads_from_of ce (e, b))) &
+           (carries_a_dependency_to ce (b, d) | (b = d)))))"
 
 
 (* N3132 6.15 Inter-thread-happens-before and happens-before *)
 definition inter_thread_happens_before where
-  "inter_thread_happens_before ap as lk sb asw dd rf sc mo ==
-     let (a, b) = ap in
-     let sw = (%app. synchronizes_with app as lk sb asw rf sc mo) in
-     let dob = (%app. dependency_ordered_before app as lk sb dd rf mo) in
-     let r = sw Un dob Un (sw O sb) in
-     ((r Un (sb O r))^*) (a, b)"
+  "inter_thread_happens_before ce ==
+     (%(a, b).
+      let r = (synchronizes_with ce) Un
+              (dependency_ordered_before ce) Un
+              ((synchronizes_with ce) O (sequenced_before_of ce)) in
+      ((r Un ((sequenced_before_of ce) O r))^*) (a, b))"
 
 definition consistent_inter_thread_happens_before where
-  "consistent_inter_thread_happens_before as lk sb asw dd rf sc mo ==
-     let ithb = (%ap. inter_thread_happens_before ap as lk sb asw dd rf sc mo) in
-     irrefl ithb"
+  "consistent_inter_thread_happens_before ce ==
+     irrefl (inter_thread_happens_before ce)"
 
 definition happens_before where
-  "happens_before ap as lk sb asw dd rf sc mo ==
-     let ithb = (%app. inter_thread_happens_before ap as lk sb asw dd rf sc mo) in
-     (sb O ithb) ap"
+  "happens_before ce == (sequenced_before_of ce) O (inter_thread_happens_before ce)"
 
 
 (* N3132 6.16 Consistent SC order *)
 definition all_sc_actions where
-  "all_sc_actions as == {a : as. (is_seq_cst a | is_lock a | is_unlock a)}"
+  "all_sc_actions ce == {a : (actions_of ce). (is_seq_cst a | is_lock a | is_unlock a)}"
 
 definition consistent_sc_order where
-  "consistent_sc_order as lk sb asw dd rf sc mo ==
-     let hb = (%ap. happens_before ap as lk sb asw dd rf sc mo) in
-     let sc_happens_before = (relation_int (all_sc_actions as) hb) in
-     let sc_mod_order = relation_int (all_sc_actions as) mo in
-     strict_total_order_over (all_sc_actions as) sc &
-     sc_happens_before <= sc &
-     sc_mod_order <= sc"
+  "consistent_sc_order ce as lk sb asw dd rf sc mo ==
+     strict_total_order_over (all_sc_actions ce) (sequential_consistency_of ce) &
+     (relation_int (all_sc_actions as) (happens_before ce)) <= (sequential_consistency_of ce) &
+     (relation_int (all_sc_actions ce) (modification_order_of ce)) <= (sequential_consistency_of ce)"
 
 
 (* N3132 6.17 Consistent modification order *)
 definition consistent_modification_order where
-  "consistent_modification_order as lk sb asw dd rf sc mo ==
-     let hb = (%ap. happens_before ap as lk sb asw dd rf sc mo) in
-     ((ALL a : as. ALL b : as. (mo (a, b) --> same_location a b)) &
-      (ALL l : locations_of as. case lk l of
+  "consistent_modification_order ce ==
+     ((ALL a. ALL b. (modification_order_of ce (a, b) --> same_location_rel (a, b))) &
+      (ALL l : locations_of (actions_of ce). case (location_typing_of ce) l of
          Atomic => (
            let as_at_l = {a. (location_of a = Some l)} in
            let writes_at_l = {a : as_at_l. (is_store a | is_atomic_store a | is_atomic_rmw a)} in
-           (strict_total_order_over writes_at_l (relation_int as_at_l mo)) &
-           ((relation_int writes_at_l hb) <= mo) &
-           ((sb O (relation_int is_fence sc) O (relation_int writes_at_l sb)) <= mo))
+           (strict_total_order_over writes_at_l (relation_int as_at_l (modification_order_of ce))) &
+           ((relation_int writes_at_l (happens_before ce)) <= (modification_order_of ce)) &
+           (((sequenced_before_of ce) O (relation_int is_fence (sequential_consistency_of ce)) O
+             (relation_int writes_at_l (sequenced_before_of ce))) <= (modification_order_of ce)))
        | _ => (
            let as_at_l = {a. (location_of a = Some l)} in
-           ((relation_int as_at_l mo) = {}))))"
+           ((relation_int as_at_l (modification_order_of ce)) = {}))))"
 
 
 (* TODO *)
 (* N3132 6.18 Visible side effects and visible sequences of side effects *)
 definition visible_side_effect where
-  "visible_side_effect ap as lk sb asw dd rf sc mo ==
-     let (a, b) = ap in
-     let hb = (%app. happens_before app as lk sb asw dd rf sc mo) in
-     (hb (a, b) &
-      is_write a & is_read b & same_location a b &
-      ~(EX c : as. (c ~= a) & (c~= b) &
-          is_write c & same_location c b &
-          hb (a, c) & hb (c, b)))"
+  "visible_side_effect ce ==
+     (%(a, b).
+      happens_before ce (a, b) &
+      is_write a & is_read b & same_location_rel (a, b) &
+      ~(EX c. (c ~= a) & (c~= b) &
+          is_write c & same_location_rel (c, b) &
+          happens_before ce (a, c) & happens_before ce (c, b)))"
 
 definition visible_sequence_of_side_effects_tail where
-  "visible_sequence_of_side_effects_tail vsse_head b as lk sb asw dd rf sc mo ==
-     let hb = (%ap. happens_before ap as lk sb asw dd rf sc mo) in
-     {c : as. mo (vsse_head, c) &
-        ~(hb (b, c)) &
-        (ALL a : as. (mo (vsse_head, a) & mo (a, c)) --> ~(hb (b, a)))}"
+  "visible_sequence_of_side_effects_tail ce vsse_head b ==
+     {c. modification_order_of ce (vsse_head, c) &
+        ~(happens_before ce (b, c)) &
+        (ALL a. (modification_order_of ce (vsse_head, a) & modification_order_of ce (a, c))
+           --> ~(happens_before ce (b, a)))}"
 
 definition visible_sequences_of_side_effects where
-  "visible_sequences_of_side_effects ==
-     (%(vsse_head, b). %as. %lk. %sb. %asw. %dd. %rf. %sc. %mo.
-        (b, if (is_at_atomic_location b lk) then
-              ({vsse_head} Un
-               visible_sequence_of_side_effects_tail vsse_head b as lk sb asw dd rf sc mo)
-            else {}))"
+  "visible_sequences_of_side_effects ce b ==
+     setsum
+       (%vsse_head. if (is_at_atomic_location ce b) then
+                       ({vsse_head} Un
+                          visible_sequence_of_side_effects_tail ce vsse_head b)
+                    else {})
+       {vsse_head : (actions_of ce). visible_side_effect ce (vssed_head, b)}"
 
 
 (* N3132 6.19 Consistent reads-from mapping *)
 definition consistent_reads_from_mapping where
-  "consistent_reads_from_mapping as lk sb asw dd rf sc mo ==
-     let hb = (%ap. happens_before ap as lk sb asw dd rf sc mo) in
-     let vse = (%ap. visible_side_effect ap as lk sb asw dd rf sc mo) in
-     let vsose = (%(vsse_head, b). visible_sequences_of_side_effects (vsse_head, b) as lk sb asw dd rf sc mo) in
-     ((ALL b : as. (is_read b & is_at_non_atomic_location b lk) -->
-                   (if (EX avse. vse (avse, b))
-                    then (EX avse. vse (avse, b) & rf (avse, b))
-                    else ~(EX a. rf (a, b)))) &
+  "consistent_reads_from_mapping ce ==
+     ((ALL b. (is_read b & is_at_non_atomic_location ce b) -->
+              (if (EX avse. visible_side_effect ce (avse, b))
+               then (EX avse. visible_side_effect ce (avse, b) & reads_from_of ce (avse, b))
+               else ~(EX a. reads_from_of ce (a, b)))) &
 
-      (ALL b : as. (is_read b & is_at_atomic_location b lk) -->
-                   (if (EX (bb, vsse) : vsose. (bb = b))
-                    then (EX (bb, vsse) : vsose.
-                          (bb = b) & (EX c : vsse. rf (c, b)))
-                    else ~(EX a. rf (a, b))))   )"(* &
+      (ALL b. (is_read b & is_at_atomic_location ce b) -->
+              (if (EX (bb, vsse) : (visible_sequences_of_side_effects ce). (bb = b))
+               then (EX (bb, vsse) : (visible_sequences_of_side_effects ce).
+                     (bb = b) & (EX c : vsse. reads_from_of ce (c, b)))
+               else ~(EX a. reads_from_of ce (a, b))))   )"(* &
 
-      (ALL (x, a) : rf.
-         ALL (y, b) : rf.
-           (hb (a, b) &
-              same_location a b & is_at_atomic_location b lk)
-                --> ((x = y) | mo (x, y))) &
+      (ALL (x, a) : (reads_from_of ce).
+         ALL (y, b) : (reads_from_of ce).
+           (happens_before ce (a, b) &
+              same_location_rel (a, b) & is_at_atomic_location ce b)
+                --> ((x = y) | modification_order_of ce (x, y))) &
 
-      (ALL (a, b) : hb.
+      (ALL (a, b) : (happens_before ce).
          ALL c.
-           (rf (c, b) &
-              is_write a & same_location a b & is_at_atomic_location b lk)
-                --> ((c = a) | mo (a, c))) &
+           (reads_from_of ce (c, b) &
+              is_write a & same_location_rel (a, b) & is_at_atomic_location ce b)
+                --> ((c = a) | modification_order_of ce (a, c))) &
 
-      (ALL (a, b) : hb.
+      (ALL (a, b) : (happens_before ce).
          ALL c.
-           (rf (c, a) &
-              is_write b & same_location a b & is_at_atomic_location a lk)
-                --> mo (c, b)) &
+           (reads_from_of ce (c, a) &
+              is_write b & same_location_rel (a, b) & is_at_atomic_location ce a)
+                --> modification_order_of ce (c, b)) &
 
-      (ALL (a, b) : rf. is_atomic_rmw b
-         --> mo (a, b)) &
+      (ALL (a, b) : (reads_from_of ce). is_atomic_rmw b
+         --> modification_order_of (a, b)) &
 
-      (ALL (a, b) : rf. is_seq_cst b
-         --> (~(is_seq_cst a)) | (relation_int (%c. is_write c & same_location b c) sc (a, b)))   )"
+      (ALL (a, b) : (reads_from_of ce). is_seq_cst b
+         --> (~(is_seq_cst a))
+             | (relation_int (%c. is_write c & same_location_rel (b, c)) sequential_consistency_of ce (a, b)))   )"
 *)
